

DS 3001 EDA Assignment Question 1

① We want to show that $m(a+b\mathbb{X}) = a+b \times m(\mathbb{X})$.

$$\text{Formula: } m(\mathbb{X}) = \frac{1}{N} \sum_{i=1}^N x_i$$

$$\begin{aligned} m(a+b\mathbb{X}) &= \frac{1}{N} \sum_{i=1}^N (a+b x_i) \\ &= \frac{1}{N} \left(\sum_{i=1}^N a + \sum_{i=1}^N b x_i \right) = \frac{1}{N} \left(\sum_{i=1}^N a + b \sum_{i=1}^N x_i \right) \\ &= \frac{1}{N} \sum_{i=1}^N a + b \cdot \frac{1}{N} \sum_{i=1}^N x_i \\ &= \frac{1}{N} (N \cdot a) + b \cdot m(\mathbb{X}) = \boxed{a + b \cdot m(\mathbb{X})} \end{aligned}$$

② We want to show that $\text{cov}(\mathbb{X}, a+b\mathbb{Y}) = b \times \text{cov}(\mathbb{X}, \mathbb{Y})$.

$$\text{Formula: } \text{cov}(\mathbb{X}, \mathbb{Y}) = \frac{1}{N} \sum_{i=1}^N (x_i - m(\mathbb{X}))(y_i - m(\mathbb{Y}))$$

$$\begin{aligned} \text{cov}(\mathbb{X}, a+b\mathbb{Y}) &= \frac{1}{N} \sum_{i=1}^N (x_i - m(\mathbb{X}))(a + b y_i - m(a + b\mathbb{Y})) \\ &= \frac{1}{N} \sum_{i=1}^N (x_i - m(\mathbb{X}))(a + b y_i - (a + b \cdot m(\mathbb{Y}))) \\ &= \frac{1}{N} \sum_{i=1}^N (x_i - m(\mathbb{X}))(a - a + b y_i - b \cdot m(\mathbb{Y})) \\ &= \frac{1}{N} \sum_{i=1}^N (x_i - m(\mathbb{X}))(b(y_i - m(\mathbb{Y}))) \\ &= b \cdot \frac{1}{N} \sum_{i=1}^N (x_i - m(\mathbb{X}))(y_i - m(\mathbb{Y})) = \boxed{b \cdot \text{cov}(\mathbb{X}, \mathbb{Y})} \end{aligned}$$

③ We want to show that

$$\text{cov}(a+bX, a+bX) = b^2 \text{cov}(X, X)$$

$$\text{and } \text{cov}(X, X) = S^2.$$

$$\text{Formulas: } \text{cov}(X, Y) = \frac{1}{N} \sum_{i=1}^N (x_i - m(X))(y_i - m(Y))$$

$$S^2 = \frac{1}{N} \sum_{i=1}^N (x_i - m(X))^2$$

$$\text{cov}(a+bX, a+bX)$$

$$= \frac{1}{N} \sum_{i=1}^N (a+bx_i - m(a+bX))(a+bx_i - m(a+bX))$$

$$= \frac{1}{N} \sum_{i=1}^N (a+bx_i - (a+b \cdot m(X)))^2$$

$$= \frac{1}{N} \sum_{i=1}^N (a+bx_i - a - b \cdot m(X))^2$$

$$= \frac{1}{N} \sum_{i=1}^N (a - a + bx_i - b \cdot m(X))^2$$

$$= \frac{1}{N} \sum_{i=1}^N (b(x_i - m(X)))^2$$

$$= \frac{1}{N} \sum_{i=1}^N b^2 (x_i - m(X))^2$$

$$= b^2 \cdot \frac{1}{N} \sum_{i=1}^N (x_i - m(X))(x_i - m(X)) = \boxed{b^2 \text{cov}(X, X)}$$

$$\text{cov}(X, X) = \frac{1}{N} \sum_{i=1}^N (x_i - m(X))(x_i - m(X))$$

$$= \frac{1}{N} \sum_{i=1}^N (x_i - m(X))^2 = S^2$$

- ④ Non-decreasing transformations:
if $x \geq x'$, then $g(x) \geq g(x')$

Median: Yes, a non-decreasing transformation of the median is the median of the transformed variable.

Taking the 2 cases we have,
 $2 + 5x$ would just scale and shift all values, so the original median would still be the median.

$\text{arcsinh}(x)$ scales down extreme values and does not change the order of the data.

In general, non-decreasing transformations do not change the order of the data, so the median will remain the median of the transformed values.

Any quantile: Since non-decreasing transformations do not change the order of the data, any quantile will remain the same quantile of the transformed values.

IQR and Range: These will not remain the same unless the non-decreasing transformation is a linear shift. (causing the differences to remain the same). For example, for $2 + x$, the IQR and range remain the same.

For $2 + 5x$, the IQR and range need to be multiplied by 5.

For $\text{arcsinh}(x)$, the transformation is non-linear so the differences between each value will change non-linearly, causing the IQR and range to change.

⑤ non-decreasing transformation $g(\cdot)$

$$m(g(\mathcal{X})) = g(m(\mathcal{X}))$$

No, for example, \log is a non-decreasing transformation/function.

Let $\mathcal{X} = \{1, 10\}$.

$$m(\log(\mathcal{X})) = \frac{\log(1) + \log(10)}{2} = 0.5$$

$$\log(m(\mathcal{X})) = \log\left(\frac{1+10}{2}\right) = \log\left(\frac{11}{2}\right) \approx 0.74$$

$$m(\log(\mathcal{X})) \neq \log(m(\mathcal{X}))$$

So, $m(g(\mathcal{X})) = g(m(\mathcal{X}))$ is not always true.